src/Arithmetic/MontgomeryReduction/WordByWord/Proofs.v
@@ -1,7 +1,9 @@
 (*** Word-By-Word Montgomery Multiplication Proofs *)
+Require Import Coq.Arith.Arith.
 Require Import Coq.ZArith.BinInt Coq.ZArith.ZArith Coq.ZArith.Zdiv Coq.micromega.Lia.
 Require Import Crypto.Util.LetIn.
 Require Import Crypto.Util.Prod.
+Require Import Crypto.Util.NatUtil.
 Require Import Crypto.Util.ZUtil.
 Require Import Crypto.Arithmetic.ModularArithmeticTheorems Crypto.Spec.ModularArithmetic.
 Require Import Crypto.Arithmetic.MontgomeryReduction.WordByWord.Definition.
@@ -24,19 +26,28 @@ Section WordByWordMontgomery.
     {small : T -> Prop}
     {eval_zero : forall n, eval (zero n) = 0}
     {small_zero : forall n, small (zero n)}
+    {numlimbs_zero : forall n, numlimbs (zero n) = n}
     {eval_div : forall v, small v -> eval (fst (divmod v)) = eval v / r}
     {eval_mod : forall v, small v -> snd (divmod v) = eval v mod r}
     {small_div : forall v, small v -> small (fst (divmod v))}
+    {numlimbs_div : forall v, numlimbs (fst (divmod v)) = pred (numlimbs v)}
     {scmul : Z -> T -> T} (* uses double-output multiply *)
     {eval_scmul: forall a v, eval (scmul a v) = a * eval v}
     {small_scmul : forall a v, 0 <= a < r -> small v -> small (scmul a v)}
+    {numlimbs_scmul : forall a v, 0 <= a < r -> numlimbs (scmul a v) = S (numlimbs v)}
     {R : positive}
-    {R_big : R > 3} (* needed for [(N + B - 1) / R <= 1] *).
+    {R_big : R > 3} (* needed for [(N + B - 1) / R <= 1] *)
+    {R_numlimbs : nat}.
   Local Notation bn := (r * R) (only parsing).
   Context
     {add : T -> T -> T} (* joins carry *)
     {eval_add : forall a b, eval (add a b) = eval a + eval b}
     {small_add : forall a b, small a -> small b -> small (add a b)}
+    {numlimbs_add : forall a b, numlimbs (add a b) = Datatypes.S (max (numlimbs a) (numlimbs b))}
+    {drop_high : T -> T}
+    {small_drop_high : forall v, small v -> small (drop_high v)}
+    {eval_drop_high : forall v, small v -> eval (drop_high v) = eval v mod bn}
+    {numlimbs_drop_high : forall v, numlimbs (drop_high v) = min (numlimbs v) (S R_numlimbs)}
     (N : T) (Npos : positive) (Npos_correct: eval N = Z.pos Npos)
     (N_lt_R : eval N < R)
     (small_N : small N)
@@ -46,24 +57,38 @@ Section WordByWordMontgomery.
     ri (ri_correct : r*ri mod (eval N) = 1 mod (eval N)).
   Context (k : Z) (k_correct : k * eval N mod r = -1).
 
+  Create HintDb push_numlimbs discriminated.
   Create HintDb push_eval discriminated.
   Local Ltac t_small :=
     repeat first [ assumption
                  | apply small_add
                  | apply small_div
                  | apply small_scmul
+                 | apply small_drop_high
                  | apply Z_mod_lt
                  | solve [ auto ]
                  | lia
-                 | progress autorewrite with push_eval ].
+                 | progress autorewrite with push_eval
+                 | progress autorewrite with push_numlimbs ].
   Hint Rewrite
        eval_zero
        eval_div
        eval_mod
        eval_add
        eval_scmul
+       eval_drop_high
        using (repeat autounfold with word_by_word_montgomery; t_small)
     : push_eval.
+  Hint Rewrite
+       numlimbs_zero
+       numlimbs_div
+       numlimbs_add
+       numlimbs_scmul
+       numlimbs_drop_high
+       using (repeat autounfold with word_by_word_montgomery; t_small)
+    : push_numlimbs.
+  Hint Rewrite <- Max.succ_max_distr pred_Sn Min.succ_min_distr : push_numlimbs.
+
 
   (* Recurse for a as many iterations as A has limbs, varying A := A, S := 0, r, bounds *)
   Section Iteration.
@@ -78,16 +103,10 @@ Section WordByWordMontgomery.
 
     Local Notation a := (@WordByWord.Definition.a T divmod A).
     Local Notation A' := (@WordByWord.Definition.A' T divmod A).
-    Local Notation S3 := (@WordByWord.Definition.S3 T divmod r scmul add N B k A S).
     Local Notation S1 := (@WordByWord.Definition.S1 T divmod scmul add B A S).
-    Local Notation cS2 := (@WordByWord.Definition.cS2 T divmod r scmul add N B k A S).
-
-    Lemma S3_nonneg : 0 <= eval S3.
-    Proof.
-      repeat autounfold with word_by_word_montgomery;
-        autorewrite with push_eval; [].
-      rewrite ?Npos_correct; Z.zero_bounds; lia.
-    Qed.
+    Local Notation S2 := (@WordByWord.Definition.S2 T divmod r scmul add N B k A S).
+    Local Notation S3 := (@WordByWord.Definition.S3 T divmod r scmul add N B k A S).
+    Local Notation S4 := (@WordByWord.Definition.S4 T divmod r scmul add drop_high N B k A S).
 
     Lemma S3_bound
       : eval S < eval N + eval B
@@ -96,19 +115,64 @@ Section WordByWordMontgomery.
       assert (Hmod : forall a b, 0 < b -> a mod b <= b - 1)
         by (intros x y; pose proof (Z_mod_lt x y); omega).
       intro HS.
-      unfold S3, WordByWord.Definition.cS2, WordByWord.Definition.S1.
+      unfold S3, WordByWord.Definition.S2, WordByWord.Definition.S1.
       autorewrite with push_eval; [].
       eapply Z.le_lt_trans.
       { transitivity ((N+B-1 + (r-1)*B + (r-1)*N) / r);
           [ | set_evars; ring_simplify_subterms; subst_evars; reflexivity ].
         Z.peel_le; repeat apply Z.add_le_mono; repeat apply Z.mul_le_mono_nonneg; try lia;
-          autounfold with word_by_word_montgomery;
+          repeat autounfold with word_by_word_montgomery;
           autorewrite with push_eval;
             try Z.zero_bounds;
             auto with lia. }
       rewrite (Z.mul_comm _ r), <- Z.add_sub_assoc, <- Z.add_opp_r, !Z.div_add_l' by lia.
       autorewrite with zsimplify.
       omega.
+    Qed.
+
+    Lemma small_A'
+      : small A'.
+    Proof.
+      repeat autounfold with word_by_word_montgomery; auto.
+    Qed.
+
+    Lemma small_S3
+      : small S3.
+    Proof. repeat autounfold with word_by_word_montgomery; t_small. Qed.
+
+    Lemma small_S4
+      : small S4.
+    Proof. apply small_drop_high, small_S3. Qed.
+
+    Lemma S3_nonneg : 0 <= eval S3.
+    Proof.
+      repeat autounfold with word_by_word_montgomery;
+        autorewrite with push_eval; [].
+      rewrite ?Npos_correct; Z.zero_bounds; lia.
+    Qed.
+
+    Lemma S4_nonneg : 0 <= eval S4.
+    Proof. unfold S4; rewrite eval_drop_high by apply small_S3; Z.zero_bounds. Qed.
+
+    Lemma S4_bound
+      : eval S < eval N + eval B
+        -> eval S4 < eval N + eval B.
+    Proof.
+      intro H; pose proof (S3_bound H); pose proof S3_nonneg.
+      unfold S4.
+      rewrite eval_drop_high by apply small_S3.
+      rewrite Z.mod_small by nia.
+      assumption.
+    Qed.
+
+    Lemma numlimbs_S4 : numlimbs S4 = min (max (1 + numlimbs S) (1 + max (1 + numlimbs B) (numlimbs N))) (1 + R_numlimbs).
+    Proof.
+      cbn [plus].
+      repeat autounfold with word_by_word_montgomery.
+      repeat autorewrite with push_numlimbs.
+      change Init.Nat.max with Nat.max.
+      rewrite <- ?(Max.max_assoc (numlimbs S)).
+      reflexivity.
     Qed.
 
     Lemma S1_eq : eval S1 = S + a*B.
@@ -118,14 +182,14 @@ Section WordByWordMontgomery.
       reflexivity.
     Qed.
 
-    Lemma cS2_mod_N : (eval cS2) mod N = (S + a*B) mod N.
+    Lemma S2_mod_N : (eval S2) mod N = (S + a*B) mod N.
     Proof.
       assert (bn_large : bn >= r) by (unfold bn; nia).
-      cbv [cS2 WordByWord.Definition.q WordByWord.Definition.s]; autorewrite with push_eval zsimplify. rewrite S1_eq. reflexivity.
+      cbv [S2 WordByWord.Definition.q WordByWord.Definition.s]; autorewrite with push_eval zsimplify. rewrite S1_eq. reflexivity.
     Qed.
 
-    Lemma cS2_mod_r : cS2 mod r = 0.
-      cbv [cS2 WordByWord.Definition.q WordByWord.Definition.s]; autorewrite with push_eval.
+    Lemma S2_mod_r : S2 mod r = 0.
+      cbv [S2 WordByWord.Definition.q WordByWord.Definition.s]; autorewrite with push_eval.
       assert (r > 0) by lia.
       assert (Hr : (-(1 mod r)) mod r = r - 1 /\ (-(1)) mod r = r - 1).
       { destruct (Z.eq_dec r 1) as [H'|H'].
@@ -161,25 +225,23 @@ Section WordByWordMontgomery.
                             cbv [Z.equiv_modulo] in HH; rewrite HH; clear HH.
       etransitivity; [rewrite (fun a => Z.mul_mod_l a ri N)|
                       rewrite (fun a => Z.mul_mod_l a ri N); reflexivity].
-      rewrite <-cS2_mod_N; repeat (f_equal; []); autorewrite with push_eval.
+      rewrite <-S2_mod_N; repeat (f_equal; []); autorewrite with push_eval.
       autorewrite with push_Zmod;
         replace (bn mod r) with 0
         by (symmetry; apply Z.mod_divide; try assumption; try lia);
-        rewrite cS2_mod_r;
+        rewrite S2_mod_r;
         autorewrite with zsimplify.
       reflexivity.
     Qed.
 
-    Lemma small_A'
-      : small A'.
+    Lemma S4_mod_N
+          (Hbound : eval S < eval N + eval B)
+      : S4 mod N = (S + a*B)*ri mod N.
     Proof.
-      repeat autounfold with word_by_word_montgomery; auto.
-    Qed.
-
-    Lemma small_S3
-      : small S3.
-    Proof.
-      repeat autounfold with word_by_word_montgomery; t_small.
+      pose proof (S3_bound Hbound); pose proof S3_nonneg.
+      unfold S4; autorewrite with push_eval.
+      rewrite (Z.mod_small _ bn) by nia.
+      apply S3_mod_N.
     Qed.
 
     Lemma small_from_bound
@@ -196,28 +258,15 @@ Section WordByWordMontgomery.
     Qed.
   End Iteration.
 
-  Local Notation redc_body := (@redc_body T divmod r scmul add N B k).
-  Local Notation redc_loop := (@redc_loop T divmod r scmul add N B k).
-  Local Notation redc A := (@redc T numlimbs zero divmod r scmul add N A B k).
-
-  Fixpoint redc_loop_rev (count : nat) : T * T -> T * T
-    := match count with
-       | O => fun A_S => A_S
-       | S count' => fun A_S => redc_body (redc_loop_rev count' A_S)
-       end.
+  Local Notation redc_body := (@redc_body T divmod r scmul add drop_high N B k).
+  Local Notation redc_loop := (@redc_loop T divmod r scmul add drop_high N B k).
+  Local Notation redc A := (@redc T numlimbs zero divmod r scmul add drop_high N A B k).
 
   Lemma redc_loop_comm_body count
     : forall A_S, redc_loop count (redc_body A_S) = redc_body (redc_loop count A_S).
   Proof.
     induction count as [|count IHcount]; try reflexivity.
     simpl; intro; rewrite IHcount; reflexivity.
-  Qed.
-
-  Lemma redc_loop__redc_loop_rev count
-    : forall A_S, redc_loop count A_S = redc_loop_rev count A_S.
-  Proof.
-    induction count as [|count IHcount]; try reflexivity.
-    simpl; intro; rewrite <- IHcount, redc_loop_comm_body; reflexivity.
   Qed.
 
   Section body.
@@ -228,19 +277,18 @@ Section WordByWordMontgomery.
     Let a:=snd A_a.
     Context (small_A : small A)
             (small_S : small S)
-            (S_nonneg : 0 <= eval S)
-            (S_div_R_small : eval S / R <= 1).
+            (S_bound : 0 <= eval S < eval N + eval B).
 
     Lemma small_fst_redc_body : small (fst (redc_body A_S)).
     Proof. destruct A_S; apply small_A'; assumption. Qed.
     Lemma small_snd_redc_body : small (snd (redc_body A_S)).
-    Proof. destruct A_S; apply small_S3; assumption. Qed.
+    Proof. destruct A_S; apply small_S4; assumption. Qed.
     Lemma snd_redc_body_nonneg : 0 <= eval (snd (redc_body A_S)).
-    Proof. destruct A_S; apply S3_nonneg; assumption. Qed.
+    Proof. destruct A_S; apply S4_nonneg; assumption. Qed.
 
     Lemma snd_redc_body_mod_N
       : (eval (snd (redc_body A_S))) mod (eval N) = (eval S + a*eval B)*ri mod (eval N).
-    Proof. destruct A_S; apply S3_mod_N; assumption. Qed.
+    Proof. destruct A_S; apply S4_mod_N; auto; omega. Qed.
 
     Lemma fst_redc_body
       : (eval (fst (redc_body A_S))) = eval (fst A_S) / r.
@@ -264,8 +312,12 @@ Section WordByWordMontgomery.
       : eval S < eval N + eval B
         -> eval (snd (redc_body A_S)) < eval N + eval B.
     Proof.
-      destruct A_S; apply S3_bound; assumption.
+      destruct A_S; apply S4_bound; unfold S in *; cbn [snd] in *; try assumption; try omega.
     Qed.
+
+    Lemma numlimbs_redc_body : numlimbs (snd (redc_body A_S))
+                               = min (max (1 + numlimbs (snd A_S)) (1 + max (1 + numlimbs B) (numlimbs N))) (1 + R_numlimbs).
+    Proof. destruct A_S; apply numlimbs_S4; assumption. Qed.
   End body.
 
   Local Arguments Z.pow !_ !_.
@@ -295,6 +347,51 @@ Section WordByWordMontgomery.
         (Hbound : 0 <= eval (snd A_S) < eval N + eval B)
     : 0 <= eval (snd (redc_loop count A_S)) < eval N + eval B.
   Proof. apply redc_loop_good; assumption. Qed.
+
+  Local Ltac t_min_max_step _ :=
+    match goal with
+    | [ |- context[Init.Nat.max ?x ?y] ]
+      => first [ rewrite (Max.max_l x y) by omega
+               | rewrite (Max.max_r x y) by omega ]
+    | [ |- context[Init.Nat.min ?x ?y] ]
+      => first [ rewrite (Min.min_l x y) by omega
+               | rewrite (Min.min_r x y) by omega ]
+    | _ => progress change Init.Nat.max with Nat.max
+    | _ => progress change Init.Nat.min with Nat.min
+    end.
+
+  Lemma numlimbs_redc_loop A_S count
+        (Hsmall : small (fst A_S) /\ small (snd A_S))
+        (Hbound : 0 <= eval (snd A_S) < eval N + eval B)
+        (Hnumlimbs : (R_numlimbs <= numlimbs (snd A_S))%nat)
+    : numlimbs (snd (redc_loop count A_S))
+      = match count with
+        | O => numlimbs (snd A_S)
+        | S _ => 1 + R_numlimbs
+        end%nat.
+  Proof.
+    assert (Hgen
+            : numlimbs (snd (redc_loop count A_S))
+              = match count with
+                | O => numlimbs (snd A_S)
+                | S _ => min (max (count + numlimbs (snd A_S)) (1 + max (1 + numlimbs B) (numlimbs N))) (1 + R_numlimbs)
+                end).
+    { induction_loop count IHcount; [ reflexivity | ].
+      rewrite numlimbs_redc_body by (try apply redc_loop_good; auto).
+      rewrite IHcount; clear IHcount.
+      destruct count; [ reflexivity | ].
+      destruct (Compare_dec.le_lt_dec (1 + max (1 + numlimbs B) (numlimbs N)) (S count + numlimbs (snd A_S))),
+      (Compare_dec.le_lt_dec (1 + R_numlimbs) (S count + numlimbs (snd A_S))),
+      (Compare_dec.le_lt_dec (1 + R_numlimbs) (1 + max (1 + numlimbs B) (numlimbs N)));
+        repeat first [ reflexivity
+                     | t_min_max_step ()
+                     | progress autorewrite with push_numlimbs
+                     | rewrite Nat.min_comm, Nat.min_max_distr ]. }
+    rewrite Hgen; clear Hgen.
+    destruct count; [ reflexivity | ].
+    repeat apply Max.max_case_strong; apply Min.min_case_strong; omega.
+  Qed.
+
 
   Lemma fst_redc_loop A_S count
         (Hsmall : small (fst A_S) /\ small (snd A_S))
@@ -372,6 +469,20 @@ Section WordByWordMontgomery.
   Proof. apply redc_good; assumption. Qed.
   Lemma redc_bound A (small_A : small A) : 0 <= eval (redc A) < eval N + eval B.
   Proof. apply redc_good; assumption. Qed.
+  Lemma numlimbs_redc_gen A (small_A : small A) (Hnumlimbs : R_numlimbs <= numlimbs B)
+    : numlimbs (redc A)
+      = match numlimbs A with
+        | O => S (numlimbs B)
+        | _ => S R_numlimbs
+        end.
+  Proof.
+    unfold redc; rewrite numlimbs_redc_loop by (cbn [fst snd]; t_small);
+      cbn [snd]; rewrite ?numlimbs_zero.
+    reflexivity.
+  Qed.
+  Lemma numlimbs_redc A (small_A : small A) (Hnumlimbs : R_numlimbs = numlimbs B)
+    : numlimbs (redc A) = S (numlimbs B).
+  Proof. rewrite numlimbs_redc_gen; subst; auto; destruct (numlimbs A); reflexivity. Qed.
 
   Lemma redc_mod_N A (small_A : small A)
     : (eval (redc A)) mod (eval N) = (eval A * eval B * ri^(Z.of_nat (numlimbs A))) mod (eval N).
